$$
f_m(x) = f_{m-1}(x) + \beta_m b(x;\gamma_m) \tag{1.0}
$$


$$
\begin{gather}
a + b = b + a + c + d \\
a + b = b + a + c + d \\
a + b = b + a + c + d \\
a + b = b + a + c + d \\
a + b = b + a + c + d 
\tag{1.1}
\end{gather}
$$


$$
\begin{align}
x &= t + \cos t + 1\\
x &= t + \cos t + 1 \\
x &= t + \cos t + 1 \\
x &= t + \cos t + 1 \\
x &= t + \cos t + 1 \\
x &= t + \cos t + 1 \\
\tag{1.2}
\end{align}
$$


$$
\begin{array}{rcr}
f(x,y,z) & = & x + y + z  \\
f(x,y,z) & = & x + y + z   \\
f(x,y,z) & = & x + y + z  \\
f(x,y,z) & = & x + y + z  \\
\tag{1.3}
\end{array}
$$


$$
\begin{matrix}
a_{11} & a_{12} & a_{13} \\
0      & a_{22} & a_{23} \\
0	   & 0      & a_{33}   
\tag{1.4}
\end{matrix}
$$



$$
\begin{align}
x = y+1 \\
y = x+2\\
z = x+2\\
m = x+2\\
\tag{2}
\end{align}
$$



##### 复杂公式设计(equation环境+array)

$$
\begin{equation}
\begin{array}{ccc}
\frac{\partial f_l(\mathbf{a}^l) }{\partial \mathbf{a}^l} &=
\begin{bmatrix}
\frac{ \partial f_l(a^l_{1})}{\partial a^l_1} & \frac{ \partial f_l(a^l_{2})}{\partial a^l_1} & \cdots & \frac{ \partial f_l(a^l_{N_l -1})}{\partial a^l_1} & \frac{ \partial f_l(1)}{\partial a^l_1} \\
\frac{ \partial f_l(a^l_{1})}{\partial a^l_2} & \frac{ \partial f_l(a^l_{2})}{\partial a^l_2} & \cdots & \frac{ \partial f_l(a^l_{N_l -1})}{\partial a^l_2} & \frac{ \partial f_l(1)}{\partial a^l_2} \\
\vdots& \vdots & \ddots & \vdots & \vdots \\
\frac{ \partial f_l(a^l_{1})}{\partial a^l_{N_l -1}} & \frac{ \partial f_l(a^l_{2})}{\partial a^l_{N_l -1}} & \cdots & \frac{ \partial f_l(a^l_{N_l -1})}{\partial a^l_{N_l -1}} & \frac{ \partial f_l(1)}{\partial a^l_{N_l -1}} \\
\frac{ \partial f_l(a^l_{1})}{\partial 1} & \frac{ \partial f_l(a^l_{2})}{\partial 1} & \cdots & \frac{ \partial f_l(a^l_{N_l -1})}{\partial 1} & \frac{ \partial f_l(1)}{\partial 1}
\end{bmatrix} \\\\
		&=
\begin{bmatrix}
\frac{ \partial f_l(a^l_{1})}{\partial a^l_1} & 0 & \cdots & 0 & 0 \\
0 & \frac{ \partial f_l(a^l_{2})}{\partial a^l_2} & \cdots & 0 & 0\\
\vdots& \vdots & \ddots & \vdots & \vdots \\
0 & 0 & \cdots & \frac{ \partial f_l(a^l_{N_l -1})}{\partial a^l_{N_l -1}} & 0 \\
0 & 0 & \cdots & 0 & 0
\end{bmatrix} \\\\
		&= A^l
\end{array}
\tag{10}
\end{equation}
$$
